doc/design/DotNet/DecidableEq.lean
@@ -53,8 +53,6 @@ theorem Pos.minus_one_eq_iff_eq (pos1 pos2: Pos) : (pos1.val - 1 = pos2.val - 1)
 end Pos
 
 
-section TypeDef
-
 instance : BEq TypeDef := inferInstance
 
 instance : LawfulBEq TypeDef := inferInstance
@@ -63,7 +61,14 @@ instance : LawfulHashable TypeDef := inferInstance
 
 instance : EquivBEq TypeDef := inferInstance
 
-end TypeDef
+
+theorem beq_iff_eq_at.{u} (α: Type u) [BEq α] [LawfulBEq α] {a b : α} : (a == b) ↔ a = b := beq_iff_eq
+
+
+theorem TypeStack.Indexless.indexed_eq
+  (tstI: Indexless)
+  : tstI.indexed = (match tstI with | .mk _ tst => tst) := by
+  rfl
 
 -- Note: 왜 함수 안에 직접 `sizeOf` 를 사용할 수 없는건데??
 @[expose]
@@ -75,6 +80,14 @@ def TypeSpec.mapConOrDefault.{u} {α: Sort u}
   | .var => fallback
   | .con tst => mapFunc tst
 
+theorem TypeSpec.mapConOrDefault_eq.{u} {α: Sort u} tsp mapFunc (fallback: α)
+  : TypeSpec.mapConOrDefault tsp mapFunc fallback
+    = (match tsp with | .var => fallback | .con tst => mapFunc tst) := by
+  rfl
+
+section extra_simp
+
+attribute [simp] TypeSpec.mapConOrDefault_eq
 
 mutual
 
@@ -98,7 +111,7 @@ open TypeStack
   termination_by
     (sizeOf tstI1.indexed, 0)
   decreasing_by
-    unfold TypeSpec.mapConOrDefault
+    simp
     next =>
       split
       next =>
@@ -108,7 +121,6 @@ open TypeStack
         simp
         decreasing_with omega
     next =>
-      simp
       unfold TypeStack.toIndexless -- Note: '보이지 않는 Term' 에서 다름이 있었다..!
       decreasing_with omega
 
@@ -123,7 +135,6 @@ open TypeStack
   termination_by
     (tsp1.mapConOrDefault sizeOf 0, 1)
   decreasing_by
-    simp only [toIndexless_indexed_eq]
     decreasing_with omega
 
 end
@@ -150,7 +161,7 @@ open TypeStack
   termination_by
     (sizeOf tstI.indexed, 0)
   decreasing_by
-    unfold TypeSpec.mapConOrDefault
+    simp
     next =>
       split
       next => simp; decreasing_with omega
@@ -201,7 +212,7 @@ open TypeStack
   termination_by
     (sizeOf tstI.indexed, 0)
   decreasing_by
-    unfold TypeSpec.mapConOrDefault
+    simp
     next =>
       split
       next =>
@@ -248,56 +259,239 @@ open TypeStack
   theorem TypeStack.Indexless.eq_of_beq
     {tst1I tst2I: Indexless} (is_beq: tst1I == tst2I)
     : tst1I = tst2I := by
-    have is_beq0 : Indexless.beq tst1I tst2I := by exact is_beq
-    obtain ⟨rc1, tst1⟩ := tst1I
-    obtain ⟨rc2, tst2⟩ := tst2I
-    simp
-    unfold Indexless.beq at is_beq0
+    rewrite [show type_of% is_beq = Indexless.beq tst1I tst2I by trivial] at is_beq
+    unfold Indexless.beq at is_beq
+    --obtain ⟨rc1, tst1⟩ := tst1I
+    --obtain ⟨rc2, tst2⟩ := tst2I
+    match arg : (tst1I, tst2I) with
+    | Prod.mk (Indexless.mk rc1 tst1) (Indexless.mk rc2 tst2) =>
+      simp at arg
+      obtain ⟨arg1, arg2⟩ := arg
+      obtain ⟨rc1i, tst1i⟩ := tst1I
+      obtain ⟨rc2i, tst2i⟩ := tst2I
+      obtain ⟨rc_eq1, tst_eq1⟩ := arg1
+      obtain ⟨rc_eq2, tst_eq2⟩ := arg2
+      simp_all
+      sorry
+
+
+
+
+
+
+
+
+
+
+
+
+
+
+/-
+      conv at is_beq =>
+        arg 1
+        rw [arg1, arg2]
+        simp
+        congr
+        next =>
+          intro td1
+          simp_match
+-/
+
+
+
+      --obtain ⟨arg1, arg2⟩ := arg
+/-
     cases tst1 with
-    | alloc _ =>
+    | alloc td1 =>
       cases tst2 with
-      | alloc _ =>
-        simp_all
-        rw [is_beq0]
+      | alloc td2 =>
+        simp [*] at *
+        congr
       | push _ _ _ =>
+        conv at is_beq =>
+          arg 1
+          rw [lm_clone.symm]
         contradiction
     | push prc1 pred1 item1 =>
       cases tst2 with
       | alloc _ =>
         contradiction
       | push prc2 pred2 item2 =>
-        simp at is_beq0
-        obtain ⟨tsp_beq, tst_beq⟩ := is_beq0
-        have lemma2 : pred1.toIndexless = pred2.toIndexless := TypeStack.Indexless.eq_of_beq (by exact tst_beq)
-        have lemma1 : item1 = item2 := TypeSpec.eq_of_beq (by exact tsp_beq)
-        unfold TypeStack.toIndexless at lemma2
-        simp at lemma2
-        obtain ⟨prc_val_eq, pred_eq⟩ := lemma2
-        simp [prc_val_eq]
+        simp_all
+        obtain ⟨tsp_beq, tst_beq⟩ := is_beq
+        have lemma1 : item1 == item2 := by exact tsp_beq
+        have lm_tsp_eq := TypeSpec.eq_of_beq lemma1
+        have lemma2 : pred1.toIndexless == pred2.toIndexless := by exact tst_beq
+        have lm_tst_eq : pred1.toIndexless = pred2.toIndexless := TypeStack.Indexless.eq_of_beq lemma2
+        unfold TypeStack.toIndexless at lm_tst_eq
+        simp at lm_tst_eq
+        obtain ⟨prc_val_eq, ptst_eq⟩ := lm_tst_eq
         have prc_eq := Subtype.ext prc_val_eq
+        simp_all
         congr
+-/
   termination_by
     (sizeOf tst1I.indexed, 0)
   decreasing_by
-    next _ heq2 =>
-      split at is_beq0
-      next _ rc2 tst1 tstI_eq =>
-        simp [*, Prod.lex_def] at *
-        obtain ⟨lhs, rhs⟩ := tstI_eq
+    --obtain ⟨rc2, tst2⟩ := tst2I
+    --obtain ⟨rc1, tst1⟩ := tst1I
+    --unfold Indexless.beq at tst_beq
+    --unfold TypeSpec.beq at tsp_beq
+    --rewrite [lm_tsp_eq] at *
+    rename ((tst2I : Indexless) ×' (tst1I == tst2I) = true) => tst2ISigma
+    have lm_tstI_eq (tstI₀1 tstI₀2: Indexless) : (tstI₀1 == tstI₀2) = (tstI₀1.beq tstI₀2) := by rfl
+    next =>
+      apply Prod.Lex.left
+      simp_all
+      --subst_eqs
+      cases item1 with
+      | var => simp; exact tst1I.indexed.sizeOf_gt_zero
+      | con tst1 =>
+        obtain ⟨rc2ᵢ, tst2ᵢ⟩ := tst2I
+        obtain ⟨rc1ᵢ, tst1ᵢ⟩ := tst1I
+        simp [lm_tstI_eq] at is_beq
+        simp [lm_tstI_eq] at tst2ISigma
+        obtain ⟨tst2ISigma_l, is_beq_s⟩ := tst2ISigma
+        obtain ⟨rc2ᵢs, tst2ᵢs⟩ := tst2ISigma_l
+        simp_all
+        unfold Indexless.beq at tst_beq
+        simp [*] at tst_beq
 
-        --simp_all
-    --unfold TypeSpec.mapConOrDefault
 
 
 
 
+    next =>
+      sorry
+
+/-
+    cases tst1 with
+    | alloc td1 =>
+      -- contradiction - unreachable
+      have lemma1 : tst1 ≍ TypeStack.alloc td1 := by trivial
+      simp_all
+      subst_eqs
+-/
+
+
+
+/-
+      cases tst2 with
+      | alloc td2 =>
+        -- contradiction - unreachable
+        simp_all
+        subst_eqs
+        rename_i cont _ _ _ _
+
+        cases item1 with
+        | var =>
+          apply Prod.Lex.left
+          simp
+          omega
+        | con tst1₁ =>
+          --contradiction
+          simp_all
+          subst_eqs
+          rename_i is_beq1 _ _ _ _ _
+          have lm_tstI_eq (tstI₀1 tstI₀2: Indexless) : (tstI₀1 == tstI₀2) = (tstI₀1.beq tstI₀2) := by rfl
+          have lm_td_eq : td1 = td2 := by
+            simp [lm_tstI_eq] at is_beq1
+            unfold Indexless.beq at is_beq1
+            simp at is_beq1
+            exact is_beq1
+          skip
+
+          cases item2 with
+          | var => contradiction
+          | con tst2₁ =>
+            apply Prod.Lex.left
+            simp_all
+            subst_eqs
+            rename_i is_beq4 _ _ is_beq3 is_beq2 is_beq1
+            have lm_td_eq : td1 = td2 := by
+              have lemma1 (tstI₀1 tstI₀2: Indexless) : (tstI₀1 == tstI₀2) = (tstI₀1.beq tstI₀2) := by rfl
+              simp [lemma1] at is_beq4
+              unfold Indexless.beq at is_beq4
+              simp at is_beq4
+              exact is_beq4
+            simp_all
+            unfold Indexless.beq at tsp_beq
+            conv at is_beq =>
+              lhs
+            --rewrite [show type_of% is_beq4 = ((TypeStack.alloc td1).toIndexless.beq (TypeStack.alloc td2).toIndexless) by trivial] at is_beq4
+            --rename ((TypeSpec.con tst1₁).beq (TypeSpec.con tst2₁) = true ∧ pred1.toIndexless.beq pred2.toIndexless = true) => is_beq₁
+            --obtain ⟨pred_beq, tst₁_con_beq⟩ := is_beq₁
+-/
+
+
+
+/-
+
+    cases item1 with
+    | var =>
+      apply Prod.Lex.left
+      simp
+      exact tst1I.indexed.sizeOf_gt_zero
+    | con tst1 =>
+      apply Prod.Lex.left
+      simp
+      cases item2 with
+      | var =>
+        contradiction
+      | con tst2 =>
+        simp
+    --rewrite [show type_of% is_beq = Indexless.beq tst1I tst2I by trivial] at is_beq
+    --unfold Indexless.beq at is_beq
+
+    obtain ⟨rc1, tst1⟩ := tst1I
+
+    obtain ⟨rc2, tst2⟩ := tst2I
+
+
+    cases tst1 with
+    | alloc td1 =>
+      cases tst2 with
+      | alloc td2 =>
+        apply Prod.Lex.left
+        simp
+        cases item1 with
+        | var =>
+          simp
+          omega
+        | con tst1₁ =>
+          simp_all
+          subst_vars
+          cases item2 with
+          | var =>
+            skip
+-/
+/-
+    cases tst1 with
+    | alloc td1 =>
+      simp only [TypeSpec.mapConOrDefault_eq]
+
+    next =>
+      sorry
+-/
+
+
+
+/-
+    match tst1I with
+    | ⟨_, .alloc td1⟩ =>
+      simp_all
+      sorry
+    | ⟨_, .push prc1 pred1 item1⟩ =>
+      sorry
+-/
 
 
 
   theorem TypeSpec.eq_of_beq
     {tsp1 tsp2: TypeSpec} (is_beq: tsp1 == tsp2) : tsp1 = tsp2 := by
-    have is_beq0 : TypeSpec.beq tsp1 tsp2 := by exact is_beq
-    unfold TypeSpec.beq at is_beq0
+    rewrite [show type_of% is_beq = TypeSpec.beq tsp1 tsp2 by trivial] at is_beq
+    unfold TypeSpec.beq at is_beq
     cases tsp1 with
     | var =>
       cases tsp2 with
@@ -307,11 +501,12 @@ open TypeStack
       cases tsp2 with
       | var => contradiction
       | con tst2 =>
-        simp at is_beq0
-        have lemma1 : tst1.toIndexless = tst2.toIndexless := TypeStack.Indexless.eq_of_beq (by exact is_beq0)
-        unfold TypeStack.toIndexless at lemma1
-        simp at lemma1
-        rw [lemma1]
+        simp at is_beq
+        have lemma1 : tst1.toIndexless == tst2.toIndexless := by exact is_beq
+        have lm_tstI_eq := TypeStack.Indexless.eq_of_beq lemma1
+        unfold TypeStack.toIndexless at lm_tstI_eq
+        simp at lm_tstI_eq
+        congr
   termination_by
     (tsp1.mapConOrDefault sizeOf 0, 1)
   decreasing_by
@@ -320,7 +515,7 @@ open TypeStack
 
 end
 
-
+end extra_simp
 
 
 end DotNet
